use section parameter and fix FilterRepr

examples/sbf/ConFilter.v
@@ -4,68 +4,70 @@ Require Import ProD3.examples.sbf.Utils.
 Import ListNotations.
 Open Scope Z_scope.
 
+Definition items (T: Type) size := { i: list T | Zlength i = size }.
+
+Program Definition map_items {A B: Type} {size}
+  (f: A -> B) (l: items A size): items B size := map f l.
+Next Obligation.
+  destruct l as [l ?H]. list_solve.
+Qed.
+
+Definition row num_slots := items bool num_slots.
+
+Definition frame num_rows num_slots := items (row num_slots) num_rows.
+
 Section ConFilter.
 
-  Definition items (T: Type) size := { i: list T | Zlength i = size }.
+Context {num_rows num_slots : Z}.
 
-  Program Definition map_items {A B: Type} {size}
-    (f: A -> B) (l: items A size): items B size := map f l.
-  Next Obligation.
-    destruct l as [l ?H]. list_solve.
-  Qed.
+Program Definition row_insert (r : row num_slots) (i : Z) : row num_slots :=
+  upd_Znth i r true.
+Next Obligation.
+  destruct r. list_solve.
+Qed.
 
-  Definition row num_slots := items bool num_slots.
+Lemma row_insert_comm : forall (r: row num_slots) x y,
+    row_insert (row_insert r x) y = row_insert (row_insert r y) x.
+Proof.
+  intros. destruct r as [r ?H]. unfold row_insert. simpl.
+  apply subset_eq_compat. list_solve.
+Qed.
 
-  Definition frame num_rows num_slots := items (row num_slots) num_rows.
+Program Definition frame_insert (f : frame num_rows num_slots)
+  (is : items Z num_rows) : frame num_rows num_slots := map2 row_insert f is.
+Next Obligation.
+  rewrite Zlength_map2. destruct is, f. simpl. lia.
+Qed.
 
-  Program Definition row_insert {num_slots} (r : row num_slots) (i : Z) : row num_slots :=
-    upd_Znth i r true.
-  Next Obligation.
-    destruct r. list_solve.
-  Qed.
+Program Definition row_clear (r : row num_slots) (i : Z) : row num_slots:=
+  upd_Znth i r false.
+Next Obligation.
+  rewrite Zlength_upd_Znth. destruct r. easy.
+Qed.
 
-  Lemma row_insert_comm {num_slots}: forall (r: row num_slots) x y,
-      row_insert (row_insert r x) y = row_insert (row_insert r y) x.
-  Proof.
-    intros. destruct r as [r ?H]. unfold row_insert. simpl.
-    apply subset_eq_compat. list_solve.
-  Qed.
+Program Definition empty_row num_slots (H: 0 < num_slots) : row num_slots :=
+  Zrepeat false num_slots.
+Next Obligation.
+  apply Zlength_Zrepeat. lia.
+Qed.
 
-  Program Definition frame_insert {num_rows num_slots} (f : frame num_rows num_slots)
-    (is : items Z num_rows) : frame num_rows num_slots := map2 row_insert f is.
-  Next Obligation.
-    rewrite Zlength_map2. destruct is, f. simpl. lia.
-  Qed.
+Program Definition frame_clear (f : frame num_rows num_slots)
+  (is : items Z num_rows) : frame num_rows num_slots:= map2 row_clear f is.
+Next Obligation.
+  rewrite Zlength_map2. destruct is, f. simpl. lia.
+Qed.
 
-  Program Definition row_clear {num_slots} (r : row num_slots) (i : Z) : row num_slots:=
-    upd_Znth i r false.
-  Next Obligation.
-    rewrite Zlength_upd_Znth. destruct r. easy.
-  Qed.
+Program Definition row_query (r : row num_slots) (i : Z) : bool :=
+  Znth i r.
 
-  Program Definition empty_row num_slots (H: 0 < num_slots) : row num_slots :=
-    Zrepeat false num_slots.
-  Next Obligation.
-    apply Zlength_Zrepeat. lia.
-  Qed.
+Lemma row_query_insert_true : forall (r: row num_slots) z,
+    0 <= z < num_slots -> row_query (row_insert r z) z = true.
+Proof.
+  intros. destruct r as [r ?H]. unfold row_query, row_insert. simpl. list_solve.
+Qed.
 
-  Program Definition frame_clear {num_rows num_slots} (f : frame num_rows num_slots)
-    (is : items Z num_rows) : frame num_rows num_slots:= map2 row_clear f is.
-  Next Obligation.
-    rewrite Zlength_map2. destruct is, f. simpl. lia.
-  Qed.
-
-  Program Definition row_query {num_slots} (r : row num_slots) (i : Z) : bool :=
-    Znth i r.
-
-  Lemma row_query_insert_true {num_slots}: forall (r: row num_slots) z,
-      0 <= z < num_slots -> row_query (row_insert r z) z = true.
-  Proof.
-    intros. destruct r as [r ?H]. unfold row_query, row_insert. simpl. list_solve.
-  Qed.
-
-  Program Definition frame_query {num_rows num_slots} (f : frame num_rows num_slots)
-    (is : list Z) : bool :=
-    fold_andb (map2 row_query f is).
+Program Definition frame_query (f : frame num_rows num_slots)
+  (is : list Z) : bool :=
+  fold_andb (map2 row_query f is).
 
 End ConFilter.
